The proof that every primitive recursive function is loop computable is finished, no sorry remains. I will have to add more comments down the line, but as of now, this first part is now completed. The next goal is to prove the converse, that is, that every loop computable funcion is primitive recursive.

Loop/Basic.lean
@@ -693,9 +693,11 @@ theorem highest_var_p_g_ge_highest_var_p_g_i {p_g : Fin n → Program} :
 
 -- -- Store X i
 def execution_from_state_comp_store_succ_m_inputs (m : Nat) (p_g : Fin n → Program) (p_f : Program) (v : VectNat (m + 1)) :
-    execution_from_state (0 :: v.toList ++ List.zeros (offset_comp (m + 1) p_g p_f - (m + 1)) ++ List.zeros (m + 1) ++ List.zeros n)
+    execution_from_state (0 :: v.toList ++ List.zeros (offset_comp (m + 1) p_g p_f - (m + 1)) ++ List.zeros (((m + 1) + n)))
     (store_X_1_to_X_succ_n (offset_comp (m + 1) p_g p_f + 1) m)
       = 0 :: v.toList ++ List.zeros (offset_comp (m + 1) p_g p_f - (m + 1)) ++ v.toList ++ List.zeros n := by
+  have := @append_zeros_addition (m + 1) n ((m + 1) + n) rfl
+  rewrite [this.symm, ←List.append_assoc]
   have h : offset_comp (m + 1) p_g p_f - (m + 1) + (m + 1) = offset_comp (m + 1) p_g p_f := by
     suffices h : offset_comp (m + 1) p_g p_f ≥ m + 1 from Nat.sub_add_cancel h
     simp_arith [offset_comp]
@@ -758,12 +760,90 @@ def compute_store_all_succ_n_g (n m : Nat) (p_g : Fin (n + 1) → Program) (p_f 
   | 0 => compute_store_g_i p_g offset_store 0
   | n + 1 => compute_store_g_i p_g offset_store 0 ++ compute_store_all_succ_n_g n m (fun i => p_g i.succ) p_f (offset_store + 1)
 
+-- compute_store_all_succ_n_g n m (fun i ↦ p_g i.succ) p_f (offset_comp m p_g p_f + m + 1)
+-- m fijo, p_f fijo, cambia p_g
+-- compute_store_all_succ_n_g n m (fun i ↦ p_g i.succ) p_f (c + m + 1)
 def execution_from_state_comp_compute_store_succ_n_g (m : Nat) (g : Fin (n + 1) → VectNat m → Nat) (p_g : Fin (n + 1) → Program)
-    (p_f : Program) (v : VectNat m) :
+    (g_h : ∀ i, cleanly_computes (p_g i) (g i)) (p_f : Program) (v : VectNat m) :
     execution_from_state (0 :: v.toList ++ List.zeros (offset_comp m p_g p_f - m) ++ v.toList ++ List.zeros (n + 1))
     (compute_store_all_succ_n_g n m p_g p_f (offset_comp m p_g p_f + m))
       = 0 :: v.toList ++ List.zeros (offset_comp m p_g p_f - m) ++ v.toList ++ (Vector.ofFn (fun i => g i v)).toList := by
-  sorry
+
+  suffices h : ∀ c s : Nat, ∀ u : VectNat s, c ≥ highest_var_p_g p_g - m →
+    execution_from_state (0 :: v.toList ++ List.zeros c ++ u.toList ++ List.zeros (n + 1))
+    (compute_store_all_succ_n_g n m p_g p_f (c + m + s))
+      = 0 :: v.toList ++ List.zeros c ++ u.toList ++ (Vector.ofFn fun i => g i v).toList from by
+    have : offset_comp m p_g p_f ≥ highest_var_p_g p_g := by simp_arith [offset_comp]
+    have r := h (offset_comp m p_g p_f - m) m v (Nat.sub_le_sub_right this m)
+    have : offset_comp m p_g p_f ≥ m := by simp_arith [offset_comp]
+    rewrite [Nat.sub_add_cancel this] at r
+    exact r
+  revert g p_g
+  induction n
+  case zero =>
+    intro g p_g g_h c s u c_h
+    dsimp [compute_store_all_succ_n_g, compute_store_g_i, concat_is_seq_execution]
+    simp [execution_from_state]
+    repeat rewrite [←List.append_assoc]
+    repeat rewrite [←List.cons_append]
+    have : 0 :: Vector.toList v = init_state v := rfl
+    rewrite [this]
+    rewrite [List.append_assoc _ u.toList]
+    have : c ≥ highest_var (p_g 0) - m := by
+      have : highest_var (p_g 0) ≤ highest_var_p_g p_g := highest_var_p_g_ge_highest_var_p_g_i 0
+      have := Nat.sub_le_sub_right this m
+      exact Nat.le_trans this c_h
+    rewrite [cleanly_computable_append_zeros_append_xs (g_h 0) (u.toList ++ [0]) v this]
+    rewrite [←List.append_assoc]
+    have : (g 0 v :: Vector.toList v ++ List.zeros c ++ Vector.toList u).length
+        = c + m + s + 1 := by simp_arith
+    rewrite [inc_X_i_X_j_adds_value this]
+    simp [clear_value, value_at_cons_zero, init_state]
+  case succ n n_ih =>
+    intro g p_g g_h c s u c_h
+    dsimp [compute_store_all_succ_n_g, compute_store_g_i, concat_is_seq_execution]
+    simp [execution_from_state]
+    repeat rewrite [←List.append_assoc]
+    repeat rewrite [←List.cons_append]
+    have : 0 :: Vector.toList v = init_state v := rfl
+    conv =>
+      lhs
+      rewrite [this]
+      rewrite [zeros_succ]
+      rfl
+    rewrite [List.append_assoc _ u.toList]
+    have : c ≥ highest_var (p_g 0) - m := by
+      have : highest_var (p_g 0) ≤ highest_var_p_g p_g := highest_var_p_g_ge_highest_var_p_g_i 0
+      have := Nat.sub_le_sub_right this m
+      exact Nat.le_trans this c_h
+    rewrite [cleanly_computable_append_zeros_append_xs (g_h 0) (u.toList ++ 0 :: List.zeros (n + 1)) v this]
+    rewrite [←List.append_assoc]
+    have : (g 0 v :: Vector.toList v ++ List.zeros c ++ Vector.toList u).length
+        = c + m + s + 1 := by simp_arith
+    rewrite [inc_X_i_X_j_adds_value this]
+    simp [clear_value, value_at_cons_zero, init_state]
+    have : g 0 v :: List.zeros (n + 1) = [g 0 v] ++ List.zeros (n + 1) := rfl
+    rewrite [this]
+    repeat rewrite [←List.append_assoc]
+    repeat rewrite [←List.cons_append]
+    rewrite [List.append_assoc _ u.toList]
+    let u' : VectNat (s + 1) := ⟨u.toList ++ [g 0 v], by simp⟩
+    have : u.toList ++ [g 0 v] = u'.toList := rfl
+    rewrite [this]
+    have lemma_1 : ∀ i : Fin (n + 1), cleanly_computes (p_g i.succ) (g i.succ) := by
+      intro i
+      exact g_h i.succ
+    have lemma_2 : c ≥ (highest_var_p_g fun i => p_g i.succ) - m := by
+      suffices h : highest_var_p_g (fun i => p_g i.succ) ≤ highest_var_p_g p_g from by
+        have := Nat.sub_le_sub_right h m
+        exact Nat.le_trans this c_h
+      have: highest_var_p_g p_g = max (highest_var (p_g 0)) (highest_var_p_g (fun i => p_g i.succ)) := rfl
+      rewrite [this]
+      simp_arith
+    have := n_ih (fun i => g i.succ) (fun i => p_g i.succ) lemma_1 c (s + 1) u' lemma_2
+    rewrite [←Nat.add_assoc] at this
+    rewrite [this]
+    simp [u']
 
 def execution_from_state_comp_clear_succ_m_inputs (m : Nat) (p_g : Fin n → Program) (p_f : Program) (v : VectNat (m + 1)) :
     execution_from_state (0 :: v.toList ++ List.zeros (offset_comp (m + 1) p_g p_f - (m + 1)) ++ v.toList ++ xs)
@@ -791,8 +871,48 @@ def execution_from_state_comp_setup_succ_n_inputs (m : Nat) (g : Fin (n + 1) →
       = 0 :: (Vector.ofFn (fun i => g i v)).toList ++ List.zeros (offset_comp m p_g p_f - (n + 1)) ++ v.toList ++ (Vector.ofFn (fun i => g i v)).toList := by
   generalize Vector.ofFn (fun i => g i v) = w
 
-
-  sorry
+  have : offset_comp m p_g p_f + m ≥ 1 := by
+    have : offset_comp m p_g p_f ≥ 1 := by simp_arith [offset_comp]
+    exact @Nat.le_add_right_of_le _ _ m this
+  rewrite [(Nat.sub_add_cancel this).symm]
+  conv =>
+    lhs
+    repeat rewrite [List.cons_append]
+    rfl
+  rewrite [setup_X_succ]
+  have h : offset_comp m p_g p_f ≥ n + 1 := by simp_arith [offset_comp]
+  conv =>
+    lhs
+    congr
+    rfl
+    congr
+    rewrite [←Nat.sub_add_cancel h]
+    rewrite [Nat.add_comm]
+    rewrite [←append_zeros_addition (n + 1) (offset_comp m p_g p_f - (n + 1))
+      (n + 1 + (offset_comp m p_g p_f - (n + 1))) rfl]
+    rewrite [List.append_assoc _ _ v.toList]
+    rfl
+    rfl
+  have : (List.zeros (offset_comp m p_g p_f - (n + 1)) ++ Vector.toList v).length
+      = m + offset_comp m p_g p_f - (n + 1) := by
+    simp_arith; rw [Nat.add_comm, ←Nat.add_sub_assoc h _]
+  have := lemma_setup (m + offset_comp m p_g p_f - (n + 1)) n
+    ⟨List.zeros (offset_comp m p_g p_f - (n + 1)) ++ Vector.toList v, this⟩
+    w
+  dsimp at this
+  suffices h' : (n + (m + offset_comp m p_g p_f - (n + 1))) = offset_comp m p_g p_f + m - 1 from by
+    rewrite [h'] at this
+    rewrite [this]
+    simp
+  rewrite [Nat.add_comm n]
+  rewrite [Nat.sub_add_eq]
+  rewrite [Nat.sub_right_comm]
+  have := @Nat.le_add_right_of_le _ _ m h
+  rewrite [Nat.add_comm _ m] at this
+  have := Nat.sub_le_sub_right this 1
+  rewrite [Nat.add_sub_cancel] at this
+  rewrite [Nat.sub_add_cancel this]
+  rw [Nat.add_comm _ m]
 
 def execution_from_state_comp_clear_succ_n_z (m : Nat) (g : Fin (n + 1) → VectNat m → Nat) (p_g : Fin (n + 1) → Program)
     (p_f : Program) (v : VectNat m) :
@@ -810,13 +930,21 @@ def execution_from_state_comp_clear_succ_n_z (m : Nat) (g : Fin (n + 1) → Vect
     exact Nat.sub_add_cancel this
   rw [clear_Z_lemma w this]
 
-def execution_from_state_comp_execute_p_f (g : Fin (n + 1) → VectNat m → Nat) (p_g : Fin (n + 1) → Program)
+def execution_from_state_comp_execute_p_f (g : Fin n → VectNat m → Nat) (p_g : Fin n → Program)
     (f_h : cleanly_computes p_f f) :
     execution_from_state (0 :: (Vector.ofFn (fun i => g i v)).toList ++ List.zeros (offset_comp m p_g p_f - n) ++ v.toList ++ List.zeros n)
       p_f =  f (Vector.ofFn (fun i => g i v)) :: (Vector.ofFn (fun i => g i v)).toList ++ List.zeros (offset_comp m p_g p_f - n) ++ v.toList ++ List.zeros n := by
   generalize Vector.ofFn (fun i => g i v) = w
-
-  sorry
+  rewrite [List.append_assoc _ v.toList]
+  have : offset_comp m p_g p_f - n ≥ highest_var p_f - n := by
+    have : offset_comp m p_g p_f ≥ highest_var p_f := by simp_arith [offset_comp]
+    exact Nat.sub_le_sub_right this n
+  have := @cleanly_computable_append_zeros_append_xs n p_f f (offset_comp m p_g p_f - n)
+    f_h (Vector.toList v ++ List.zeros n) w this
+  dsimp [init_state] at this
+  repeat rewrite [List.cons_append]
+  rewrite [this]
+  simp
 
 def execution_from_state_comp_clear_succ_n_inputs (m : Nat) (g : Fin (n + 1) → VectNat m → Nat) (p_g : Fin (n + 1) → Program)
     (p_f : Program) (v : VectNat m) :
@@ -1191,6 +1319,108 @@ def highest_var_comp_program (g : Fin n → VectNat m → Nat) (f_h : cleanly_co
 -- 8. def execution_from_state_comp_setup_succ_m_inputs
 -- def execution_from_state_comp_clear_succ_m_z
 
+
+-- Easy theorem, but convoluted. I could fix it to make it shorter, but what
+-- matters is not the length of the proof, but the fact that the proof is
+-- valid.
+theorem execution_from_state_comp (g : Fin n → VectNat m → Nat) (f_h : cleanly_computes p_f f) (p_g : Fin n → Program)
+    (g_h : ∀ i, cleanly_computes (p_g i) (g i)) (v : VectNat m):
+   execution_from_state (init_state v ++ List.zeros (offset_comp m p_g p_f - m) ++ List.zeros (m + n))
+     (comp_program g f_h p_g g_h) =
+    f (Vector.ofFn fun i => g i v) :: Vector.toList v ++ List.zeros (offset_comp m p_g p_f - m) ++ List.zeros (m + n) := by
+  cases n
+  · cases m
+    · dsimp [init_state, comp_program]
+      have h := @execution_from_state_comp_execute_p_f _ _ p_f f v g p_g f_h
+      simp
+      simp at h
+      rw [h]
+    · dsimp [init_state, comp_program, concat_is_seq_execution]
+      simp [execution_from_state]
+      repeat rewrite [←List.cons_append]
+      have := @execution_from_state_comp_store_succ_m_inputs _ _ p_g p_f v
+      simp at this
+      repeat rewrite [←List.cons_append] at this
+      rewrite [this]
+      have := @execution_from_state_comp_clear_succ_m_inputs _ [] _ p_g p_f v
+      simp at this
+      repeat rewrite [←List.cons_append] at this
+      rewrite [this]
+      have := @execution_from_state_comp_execute_p_f _ _ p_f f v g p_g f_h
+      simp at this
+      repeat rewrite [←List.cons_append] at this
+      rewrite [this]
+      have := @execution_from_state_comp_setup_succ_m_inputs _ (f (Vector.ofFn fun i => g i v)) _ p_g p_f v
+      simp at this
+      repeat rewrite [←List.cons_append] at this
+      rewrite [this]
+      have := @execution_from_state_comp_clear_succ_m_z _ (f (Vector.ofFn fun i => g i v)) _ p_g p_f v
+      simp at this
+      repeat rewrite [←List.cons_append] at this
+      rw [this]
+  · cases m
+    · dsimp [init_state, comp_program, concat_is_seq_execution]
+      simp [execution_from_state]
+      have := @execution_from_state_comp_compute_store_succ_n_g _ _ g p_g g_h p_f v
+      simp at this
+      repeat rewrite [←List.cons_append] at this
+      rewrite [this]
+      have := @execution_from_state_comp_setup_succ_n_inputs _ _ g p_g p_f v
+      simp at this
+      repeat rewrite [←List.cons_append] at this
+      rewrite [this]
+      have := @execution_from_state_comp_clear_succ_n_z _ _ g p_g p_f v
+      simp at this
+      repeat rewrite [←List.cons_append] at this
+      rewrite [this]
+      have := @execution_from_state_comp_execute_p_f _ _ p_f f v g p_g f_h
+      simp at this
+      repeat rewrite [←List.cons_append] at this
+      rewrite [this]
+      have := @execution_from_state_comp_clear_succ_n_inputs _ (f (Vector.ofFn fun i => g i v)) _ g p_g p_f v
+      simp at this
+      repeat rewrite [←List.cons_append] at this
+      rw [this]
+    · dsimp [init_state, comp_program, concat_is_seq_execution]
+      simp [execution_from_state]
+      repeat rewrite [←List.cons_append]
+      have := @execution_from_state_comp_store_succ_m_inputs _ _ p_g p_f v
+      simp at this
+      repeat rewrite [←List.cons_append] at this
+      rewrite [this]
+      have := @execution_from_state_comp_compute_store_succ_n_g _ _ g p_g g_h p_f v
+      simp at this
+      repeat rewrite [←List.cons_append] at this
+      rewrite [this]
+      have := @execution_from_state_comp_clear_succ_m_inputs _ (Vector.ofFn fun i => g i v).toList _ p_g p_f v
+      simp at this
+      repeat rewrite [←List.cons_append] at this
+      rewrite [this]
+      have := @execution_from_state_comp_setup_succ_n_inputs _ _ g p_g p_f v
+      simp at this
+      repeat rewrite [←List.cons_append] at this
+      rewrite [this]
+      have := @execution_from_state_comp_clear_succ_n_z _ _ g p_g p_f v
+      simp at this
+      repeat rewrite [←List.cons_append] at this
+      rewrite [this]
+      have := @execution_from_state_comp_execute_p_f _ _ p_f f v g p_g f_h
+      simp at this
+      repeat rewrite [←List.cons_append] at this
+      rewrite [this]
+      have := @execution_from_state_comp_clear_succ_n_inputs _ (f (Vector.ofFn fun i => g i v)) _ g p_g p_f v
+      simp at this
+      repeat rewrite [←List.cons_append] at this
+      rewrite [this]
+      have := @execution_from_state_comp_setup_succ_m_inputs _ (f (Vector.ofFn fun i => g i v)) _ p_g p_f v
+      simp at this
+      repeat rewrite [←List.cons_append] at this
+      rewrite [this]
+      have := @execution_from_state_comp_clear_succ_m_z _ (f (Vector.ofFn fun i => g i v)) _ p_g p_f v
+      simp at this
+      repeat rewrite [←List.cons_append] at this
+      rw [this]
+
 theorem comp_is_loop_computable_cleanly (g : Fin n → VectNat m → Nat) :
       loop_computable_cleanly f
     → (∀ i, loop_computable_cleanly (g i))
@@ -1210,16 +1440,13 @@ theorem comp_is_loop_computable_cleanly (g : Fin n → VectNat m → Nat) :
   simp_arith
   rewrite [←append_zeros_addition (offset_comp m p_g p_f - m) (m + n)
      (offset_comp m p_g p_f - m + (m + n)) rfl]
-  -- rewrite [←append_zeros_addition m n (m + n) rfl]
   repeat rewrite [←List.append_assoc]
   repeat rewrite [←List.cons_append]
-
-  sorry
+  rw [execution_from_state_comp]
 
 end comp_is_loop_computable_cleanly_proof
 
 
-/-
 theorem primrec_is_loop_computable_cleanly : Nat.Primrec' f → loop_computable_cleanly f := by
   intro h
   induction h
@@ -1236,4 +1463,3 @@ theorem primrec_is_loop_computable {f : VectNat n → Nat} :
   have := primrec_is_loop_computable_cleanly this
   have := loop_computable_cleanly_is_loop_computable this
   assumption
--/
